src3.0/SoftBound/sb_def.v
@@ -581,7 +581,7 @@ Inductive sInsn_delta : Config -> State -> State -> Prop :=
          ::EC) Mem MM)
 
 | sExCall : forall S TD Ps F B lc rm gl fs rid noret ca fid fv lp cs tmn EC dck
-           gvss fptr fptrs rt fa ft la va Mem als oresult Mem' lc' rm' MM gvs,
+        gvss fptr fptrs rt fa ft la va Mem als oresult Mem' lc' rm' MM gvs,
   (* only look up the current module for the time being, 
      do not support linkage. 
      FIXME: should add excall to trace
@@ -592,7 +592,8 @@ Inductive sInsn_delta : Config -> State -> State -> Prop :=
     Some (fdec_intro (fheader_intro fa rt fid la va) dck) ->
   Opsem.params2GVs TD lp lc gl = Some gvss ->
   gvs @@ gvss ->
-  callExternalFunction Mem fid gvs = Some (oresult, Mem') ->
+  external_intrinsics.callExternalOrIntrinsics 
+    TD Mem fid dck gvs = Some (oresult, Mem') ->
   exCallUpdateLocals TD ft noret rid oresult lc rm = Some (lc',rm') ->
   sInsn_delta (mkCfg S TD Ps gl fs)  
     (mkState  
