src3.0/SoftBound/sb_ds_trans_axioms.v
@@ -198,8 +198,9 @@ Axiom set_mmetadata_fn__prop : forall TD Mem1 lc2 als2 Mem2 S2 Ps2 F2
   (forall b2, Mem.valid_block Mem1 b2 -> Mem.valid_block Mem2 b2) /\
   (forall b0, Mem.bounds Mem1 b0 = Mem.bounds Mem2 b0).
 
-Axiom dstk_spec : forall M, 
-  OpsemAux.callExternalFunction M dstk_fid nil = Some (None, M).
+Axiom dstk_spec : forall TD M, 
+  external_intrinsics.callExternalOrIntrinsics TD M dstk_fid 
+    (deckind_external eid_other) nil = Some (None, M).
 
 Axiom dstk_is_found : forall TD Ps gl lc fs, 
   exists fv,
@@ -215,16 +216,16 @@ Axiom stk_ret_sim : forall TD M1 M2 mi mgb MM bgv egv,
   mem_simulation mi TD mgb MM M1 M2 ->
   wf_sb_mi mgb mi M1 M2 ->
   exists M2',  exists M2'',
-    OpsemAux.callExternalFunction M2 ssb_fid (bgv::int2GV 0%Z::nil) = 
-      Some (None, M2') /\
-    OpsemAux.callExternalFunction M2' sse_fid (egv::int2GV 0%Z::nil) = 
-      Some (None, M2'') /\
+    external_intrinsics.callExternalOrIntrinsics TD M2 ssb_fid 
+      (deckind_external eid_other) (bgv::int2GV 0%Z::nil) = Some (None, M2') /\
+    external_intrinsics.callExternalOrIntrinsics TD M2' sse_fid 
+      (deckind_external eid_other) (egv::int2GV 0%Z::nil) = Some (None, M2'') /\
     mem_simulation mi TD mgb MM M1 M2'' /\
     wf_sb_mi mgb mi M1 M2'' /\
-    OpsemAux.callExternalFunction M2'' gsb_fid [int2GV 0%Z] = 
-      Some (Some bgv, M2'') /\
-    OpsemAux.callExternalFunction M2'' gse_fid [int2GV 0%Z] = 
-      Some (Some egv, M2'').
+    external_intrinsics.callExternalOrIntrinsics TD M2'' gsb_fid 
+      (deckind_external eid_other) [int2GV 0%Z] = Some (Some bgv, M2'') /\
+    external_intrinsics.callExternalOrIntrinsics TD M2'' gse_fid 
+      (deckind_external eid_other) [int2GV 0%Z] = Some (Some egv, M2'').
 
 Axiom ssb_is_found : forall TD Ps gl lc fs, 
   exists fv,
@@ -255,14 +256,18 @@ Axiom gse_is_found : forall TD Ps gl lc fs,
       (deckind_external eid_other)).
 
 Axiom free_doesnt_change_gsb : forall TD M1 z gv M2 als,
-  OpsemAux.callExternalFunction M1 gsb_fid [int2GV z] = ret (ret gv, M1) ->
+  external_intrinsics.callExternalOrIntrinsics TD M1 gsb_fid 
+    (deckind_external eid_other) [int2GV z] = ret (ret gv, M1) ->
   free_allocas TD M1 als = ret M2 ->
-  OpsemAux.callExternalFunction M2 gsb_fid [int2GV z] = ret (ret gv, M2).
+  external_intrinsics.callExternalOrIntrinsics TD M2 gsb_fid 
+    (deckind_external eid_other) [int2GV z] = ret (ret gv, M2).
 
 Axiom free_doesnt_change_gse : forall TD M1 z gv M2 als,
-  OpsemAux.callExternalFunction M1 gse_fid [int2GV z] = ret (ret gv, M1) ->
+  external_intrinsics.callExternalOrIntrinsics TD M1 gse_fid 
+    (deckind_external eid_other) [int2GV z] = ret (ret gv, M1) ->
   free_allocas TD M1 als = ret M2 ->
-  OpsemAux.callExternalFunction M2 gse_fid [int2GV z] = ret (ret gv, M2).
+  external_intrinsics.callExternalOrIntrinsics TD M2 gse_fid 
+    (deckind_external eid_other) [int2GV z] = ret (ret gv, M2).
 
 Axiom wrapper_fid_is_identical : forall fid, wrapper_fid fid = fid.
 
@@ -325,7 +330,8 @@ Axiom shadow_stack_exfdec : forall la lc' mi lc2 lp cs1 nts los fptr
   wf_sb_mi mgb mi Mem0 M2 /\
   mem_simulation mi (los, nts) mgb MM Mem0 M2 /\
   reg_simulation mi (los, nts) gl2 (fdef_intro fh1 bs1) rm rm2 lc lc2 ->
-  OpsemAux.callExternalFunction Mem0 fid gvs = ret (oresult, Mem') ->
+  external_intrinsics.callExternalOrIntrinsics (los,nts) Mem0 fid 
+    dck gvs = ret (oresult, Mem') ->
   SBspec.exCallUpdateLocals (los, nts) ft noret0 rid oresult lc rm = 
     ret (lc', rm') ->
   ret cs1 = trans_params rm2 lp 1 ->
@@ -351,13 +357,17 @@ Axiom shadow_stack_exfdec : forall la lc' mi lc2 lp cs1 nts los fptr
 
 Axiom free_allocas_preserves_gsb : forall M2 TD als2 M2' lp re,
   free_allocas TD M2 als2 = ret M2' ->
-  OpsemAux.callExternalFunction M2 gsb_fid lp = Some (re, M2) ->
-  OpsemAux.callExternalFunction M2' gsb_fid lp = Some (re, M2').
+  external_intrinsics.callExternalOrIntrinsics TD M2 gsb_fid 
+    (deckind_external eid_other) lp = Some (re, M2) ->
+  external_intrinsics.callExternalOrIntrinsics TD M2' gsb_fid 
+    (deckind_external eid_other) lp = Some (re, M2').
 
 Axiom free_allocas_preserves_gse : forall M2 TD als2 M2' lp re,
   free_allocas TD M2 als2 = ret M2' ->
-  OpsemAux.callExternalFunction M2 gse_fid lp = Some (re, M2) ->
-  OpsemAux.callExternalFunction M2' gse_fid lp = Some (re, M2').
+  external_intrinsics.callExternalOrIntrinsics TD M2 gse_fid 
+    (deckind_external eid_other) lp = Some (re, M2) ->
+  external_intrinsics.callExternalOrIntrinsics TD M2' gse_fid 
+    (deckind_external eid_other) lp = Some (re, M2').
 
 Axiom store_doesnt_change_gmmd : forall M2 b2 ofs v0 Mem2' lc2 gl als
    bid0 eid0 bgv' egv' fs F B cs tmn S Ps EC TD v ck,
