src3.0/Vellvm/external_intrinsics.v
@@ -1,0 +1,73 @@
+Require Import Ensembles.
+Require Import syntax.
+Require Import infrastructure.
+Require Import List.
+Require Import Arith.
+Require Import monad.
+Require Import trace.
+Require Import Metatheory.
+Require Import genericvalues.
+Require Import alist.
+Require Import Values.
+Require Import Memory.
+Require Import Integers.
+Require Import Coqlib.
+Require Import targetdata.
+Require Import infrastructure_props.
+Require Import typings.
+
+Import LLVMsyntax.
+Import LLVMtd.
+Import LLVMinfra.
+Import LLVMgv.
+Import LLVMtypings.
+
+(* FIXME: Because memory only stores concrete values, the semantics branches when
+   storing data. However, at rule malloc/free/load/store/call/..., the rules also 
+   branch. Thoses rules should do what bop/fop/trunc do by lifting det-rules to 
+   non-det rules!!! *)
+
+Axiom callExternalFunction : mem -> id -> list GenericValue -> 
+  option ((option GenericValue)*mem).
+
+Axiom callIntrinsics : mem -> intrinsic_id -> list GenericValue -> 
+  option ((option GenericValue)*mem).
+
+Definition callMalloc (TD:TargetData) (M:mem) (parameters: list GenericValue) 
+  : option ((option GenericValue)*mem) :=
+match parameters with
+| gn::_ => 
+    match malloc TD M Size.One gn Align.Four with
+    | Some (M', mb) => Some (Some (blk2GV TD mb), M')
+    | _ => None
+    end
+| _ => 
+   (* We should prove that given a well-formed program, this case won't happen
+      because malloc must have one parameters *)
+   None
+end.
+
+Definition callFree (TD:TargetData) (M:mem) (parameters: list GenericValue) 
+  : option ((option GenericValue)*mem) :=
+match parameters with
+| ptr::_ => 
+    match free TD M ptr with
+    | Some M' => Some (None, M')
+    | _ => None
+    end
+| _ => 
+   (* We should prove that given a well-formed program, this case won't happen
+      because free must have one parameters *)
+   None
+end.
+
+Definition callExternalOrIntrinsics (TD:TargetData) (M:mem) (fid:id) 
+  (dck:deckind) (parameters: list GenericValue) 
+  : option ((option GenericValue)*mem) :=
+match dck with
+| deckind_intrinsic iid => callIntrinsics M iid parameters
+| deckind_external eid_malloc => callMalloc TD M parameters   
+| deckind_external eid_free => callFree TD M parameters
+| deckind_external eid_other => callExternalFunction M fid parameters
+end.
+
